Arithmetic: separate facts from lemmas

Arithmetic/theories/Languages/Semantics.v
@@ -1,45 +1,79 @@
-Require Import Coq.Program.Equality. (* axiom eq_rect_eq *)
+From Coq Require Import List.
+From RAC Require Import Utils Environnement.
 From RAC.Languages Require Import Syntax.
 From RAC.Languages Require Export MiniC.Semantics MiniGMP.Semantics MiniFSL.Semantics.
 
 #[local] Open Scope c_sem_scope.
+#[local] Open Scope utils_scope.
 
 
+Import FunctionalEnv Domain.
 
-Fact ty_int_gmp_c_exp_equiv {ext_exp} (e:gmp_exp): forall env v, 
-    ty e = C_Int -> 
-    (env |= gmp_exp_to_c_exp e => v)%csem <-> generic_exp_sem env e v (ext_exp:=ext_exp).
-Proof with eauto with rac_hint.
-    intros env v Hint. split; intro H.
-    - dependent induction H; destruct e eqn:E; simpl in *; subst; try congruence; injection x as Hz; subst.
-        1,2: now constructor.
-        1,2,3: destruct (ty g1) eqn:TG1; try discriminate ; destruct (ty g2) eqn:TG2; try discriminate...
-    - induction H ; simpl in *.
-        1,2: now repeat constructor.
-        1,2,3: destruct (ty e) eqn:TE1; try discriminate ; destruct (ty e') eqn:TE2; try discriminate; econstructor.
-        1,3,6: now apply IHgeneric_exp_sem1.
-        1,2,4: now apply IHgeneric_exp_sem2.
-        1,2: assumption.
-Qed.
-
-
-
-Definition c_decl_to_gmp_decl (d:@_c_decl Empty_set) : gmp_decl := 
-    let '(C_Decl t id) := d in C_Decl (c_t_to_gmp_t t) id
+Fixpoint flatten {S T}  (s: @_c_statement S T) : list (@_c_statement S T) := match s with
+| Seq s1 s2 => flatten s1 ++ flatten s2
+| Skip => nil
+| _ => s::nil
+end
 .
 
-Fixpoint c_exp_to_gmp_exp (e:c_exp) : gmp_exp := match e with
-    | Zm z => Zm z
-    | C_Id var t => C_Id var (c_t_to_gmp_t t) 
-    | BinOpInt le op re => 
-        let (le,re) := (c_exp_to_gmp_exp le,c_exp_to_gmp_exp re) in
-        BinOpInt le op re
-    | BinOpBool le op re => 
-        let (le,re) := (c_exp_to_gmp_exp le,c_exp_to_gmp_exp re) in
-        BinOpBool le op re
-    end
+Definition unflatten {S T}  : list (@_c_statement S T) -> @_c_statement S T := fun l =>
+    List.fold_left (fun new_s  s => Seq new_s s) l Skip
+.
+
+
+(* [between left x right s] means [x] is between [left] and [right] inside [s] *)
+
+Inductive between : gmp_statement -> gmp_statement -> gmp_statement -> gmp_statement ->  Prop :=
+| Between_base : forall s1 s s2 s_whole, 
+    flatten s_whole = flatten s1 ++ flatten s ++ flatten s2 -> 
+    between s1 s s2 s_whole
+| Between_add_l s1 s_whole : forall s1' s s2 s_whole',
+    between s1 s s2 s_whole ->
+    flatten s_whole' = flatten s1'++ flatten s_whole ->
+    between s1' s s2 s_whole'
+
+| Between_add_r s2 s_whole : forall s1 s  s2' s_whole',
+    between s1 s s2 s_whole ->
+    flatten s_whole' = flatten s_whole ++ flatten s2' ->
+    between s1 s s2' s_whole' 
 .
 
 
 
+Definition In_stmt {S T} (s s' : @_c_statement S T) : Prop := List.In s (flatten s').
 
+
+Definition Forall_routines {F S T } (pgrm : @_c_program F S T) 
+    (PFuns : @_c_decl T * -> @_c_decl T * -> @_c_statement S T  -> Prop)
+    (* (PLFun : fsl_statement -> Prop)
+    (PPred : fsl_statement -> Prop) *)
+    : Prop :=
+    List.Forall (fun f => match f with
+        | PFun _ _ args decls body => PFuns args decls body
+        (* | F_Ext (LFun _ _ _ _) => True
+        | F_Ext (Predicate _ _ _) => True *)
+        | _ => True
+        end
+    ) (snd pgrm)
+.
+
+
+(* 
+    well_formed_program :
+    - all variables declared before usage
+    - all functions defined before called
+    - well typed
+*)
+Definition well_formed_pgrm (P : fsl_pgrm) (env : Env) (fenv: @fenv _fsl_statement Empty_set) := 
+    Forall_routines P ( fun args decls b =>
+        (* all used variables are declared *)
+        (forall v, List.In v (fsl_stmt_vars b) -> v ∈ env) /\ 
+        (* all functions are defined before being called *)
+        (forall rvar fname args, 
+            @In_stmt _fsl_statement Empty_set (FCall rvar fname args) b -> 
+            fname ∈ fenv.(funs)
+        
+        ) /\
+        True (* fixme: well typed ? *)
+    )
+.
