Arithmetic/theories/Languages/Lemmas.v
@@ -1,1 +1,62 @@
-From RAC.Languages Require Export MiniC.Lemmas MiniGMP.Lemmas MiniFSL.Lemmas.
+From Coq Require Import String.
+From RAC Require Import Utils.
+From RAC.Languages Require Import Syntax Semantics.  
+From RAC.Languages Require Export MiniC.Facts MiniC.Lemmas MiniGMP.Facts MiniGMP.Lemmas.
+
+
+
+
+(* Additionnal facts *)
+
+Fact mpz_exp_is_var : forall (e:_c_exp), ty e = T_Ext Mpz ->  exists x, (e = C_Id x (T_Ext Mpz))%type.
+Proof. 
+    intros. destruct e eqn:E.
+    3,4: simpl in H ; destruct (ty _c1); try congruence; destruct (ty _c2); congruence.  
+    - now exists EmptyString. 
+    - exists var. unfold Syntax.ty in H. now rewrite H. 
+Qed.
+
+
+From Coq Require Import Program.Equality. (* axiom eq_rect_eq *)
+
+
+Fact ty_int_gmp_c_exp_equiv {ext_exp} (e:gmp_exp): forall env v, 
+    ty e = C_Int -> 
+    (env |= gmp_exp_to_c_exp e => v)%csem <-> generic_exp_sem env e v (ext_exp:=ext_exp).
+Proof with eauto with rac_hint.
+    intros env v Hint. split; intro H.
+    - dependent induction H; destruct e eqn:E; simpl in *; subst; try congruence; injection x as Hz; subst.
+        1,2: now constructor.
+        1,2,3: destruct (ty g1) eqn:TG1; try discriminate ; destruct (ty g2) eqn:TG2; try discriminate...
+    - induction H ; simpl in *.
+        1,2: now repeat constructor.
+        1,2,3: destruct (ty e) eqn:TE1; try discriminate ; destruct (ty e') eqn:TE2; try discriminate; econstructor.
+        1,3,6: now apply IHgeneric_exp_sem1.
+        1,2,4: now apply IHgeneric_exp_sem2.
+        1,2: assumption.
+Qed.
+
+
+Fact flatten_noseq_noskip {S T} s : List.Forall (fun i => i <> Skip /\ forall s1 s2, i <> @Seq S T s1 s2) (@flatten S T s).
+Admitted.
+
+Fact flatten_unflatten {S T} {ext_exp} {ext_stmt} {ext_stmt_vars} : forall f e e' s, 
+    @generic_stmt_sem S T ext_exp ext_stmt ext_stmt_vars f e s e' ->
+    @generic_stmt_sem S T ext_exp ext_stmt ext_stmt_vars f e (unflatten (flatten s)) e.
+Admitted.
+
+Fact flatten_unique {S T} {ext_exp} {ext_stmt} {ext_stmt_vars} : forall s s' f e e', 
+    flatten s = flatten s' ->
+    @generic_stmt_sem S T ext_exp ext_stmt ext_stmt_vars f e s e' ->
+    @generic_stmt_sem S T ext_exp ext_stmt ext_stmt_vars f e s' e'.
+Proof.
+Admitted.
+
+Fact gmp_exp_c_exp_same_exp_vars e : exp_vars (gmp_exp_to_c_exp e) = exp_vars e.
+Proof. 
+    induction e.
+    - reflexivity.
+    - destruct ty ;  reflexivity.
+    - simpl. rewrite IHe1,IHe2. reflexivity.
+    - simpl. rewrite IHe1,IHe2. reflexivity.
+Qed.
