Arithmetic/theories/Languages/MiniC/Facts.v
@@ -1,0 +1,130 @@
+From Coq Require Import FinFun.
+From RAC Require Import Utils Environnement.
+From RAC.Languages Require Import Syntax MiniC.Semantics.
+
+Import FunctionalEnv Domain Facts.
+
+Fact untouched_var_same_eval_exp {T : Set} : forall exp_sem, 
+    _untouched_var_same_eval_exp exp_sem ->
+    _untouched_var_same_eval_exp (@generic_exp_sem T exp_sem).
+Proof with eauto with rac_hint.
+    intros exp_sem Hext ev e v x Hnotin Hderiv. induction Hderiv ; simpl in Hnotin...
+    - split... constructor. simpl. apply p_map_not_same_eq...
+    - rewrite List.in_app_iff in Hnotin ; apply Decidable.not_or_iff in Hnotin as [Hxnotine Hxnotine'].  split ; 
+        intro x';  econstructor...
+        + apply IHHderiv1...
+        + apply IHHderiv2...
+        + apply IHHderiv1...
+        + apply IHHderiv2...
+    - rewrite List.in_app_iff in Hnotin ; apply Decidable.not_or_iff in Hnotin as [Hxnotine Hxnotine'].  split ; 
+        intro x';  econstructor...
+        + apply IHHderiv1...
+        + apply IHHderiv2...
+        + apply IHHderiv1...
+        + apply IHHderiv2...
+    - rewrite List.in_app_iff in Hnotin ; apply Decidable.not_or_iff in Hnotin as [Hxnotine Hxnotine'].  split ; 
+        intro x';  econstructor...
+        + apply IHHderiv1...
+        + apply IHHderiv2...
+        + apply IHHderiv1...
+        + apply IHHderiv2... 
+Qed.
+
+Fact untouched_var_same_eval_stmt {S T : Set} : 
+    forall exp_sem stmt_sem ext_stmt_vars, 
+    _untouched_var_same_eval_stmt exp_sem stmt_sem ext_stmt_vars ->
+    _untouched_var_same_eval_stmt exp_sem (@generic_stmt_sem S T exp_sem stmt_sem ext_stmt_vars) ext_stmt_vars.
+Proof.
+    intros exp_sem stmt_sem ext_stmt_vars Hext f ev ev' s x Hderiv [Hnotin Huservar]. induction Hderiv ; simpl in Hnotin; trivial.
+    - subst. apply Decidable.not_or_iff in Hnotin as [Hdiffxresf]. simpl. autounfold with rac_hint. rewrite p_map_not_same.
+        * easy.
+        * congruence.
+    -  apply IHHderiv. 
+        intro Hcontra. apply Hnotin. apply List.in_app_iff. right. 
+        apply List.in_app_iff. now left.
+    - apply IHHderiv. intro Hcontra. apply Hnotin. apply List.in_app_iff. right. 
+        apply List.in_app_iff. now right.
+    - apply IHHderiv. simpl. intro contra. rewrite List.app_nil_r in contra. apply Hnotin. apply List.in_app_iff in contra as [Hine | Hinses].
+        * apply List.in_app_iff. now left.
+        * apply List.in_app_iff in Hinses as [Hins | Hins].
+            + apply List.in_app_iff. now right.
+            + assumption.
+    - destruct IHHderiv.
+        + intro Hcontra. apply Hnotin. apply  List.in_app_iff. now left.
+        + apply IHHderiv0. intro Hcontra. apply Hnotin. apply List.in_app_iff. now right.
+    - simpl. symmetry. apply p_map_not_same_eq ; auto.
+    (* return *)
+    - simpl. destruct (eq_dec res_f x). subst. 
+        * discriminate.
+        * autounfold with rac_hint. symmetry. rewrite p_map_not_same_eq. auto. congruence.  
+    - eapply Hext in H ; eauto.
+Qed.
+
+Fact determinist_exp_eval {T : Set}: 
+forall ext_exp_sem, _determinist_exp_eval ext_exp_sem -> _determinist_exp_eval (@generic_exp_sem T ext_exp_sem).
+Proof.
+    intros ext_exp_sem ext_inj. unfold _determinist_exp_eval. intros e. induction e ; intros ; inversion H ; inversion H0 ; subst ; try easy.
+    4,5:
+        apply IHe1 with (v:=VInt (z ⁱⁿᵗ z_ir)) (v':=VInt (z0 ⁱⁿᵗ z_ir0)) in H11 ; [|assumption] ; injection H11 as eqz ;
+        apply IHe2 with (v:=VInt (z' ⁱⁿᵗ z'_ir)) (v':= VInt (z'0 ⁱⁿᵗ z'_ir0)) in H13; [|assumption] ;  injection H13 as eqz' ; subst ; now rewrite H14 in H7.
+    - f_equal. f_equal. now apply Int.mi_eq. 
+    - congruence.
+    - f_equal. f_equal. apply Int.mi_eq. simpl. f_equal.
+        + apply IHe1 with (v:=VInt (z ⁱⁿᵗ z_ir)) (v':= VInt (z0 ⁱⁿᵗ z_ir0)) in H13; [|assumption]. now injection H13. 
+        + apply IHe2 with (v:=VInt (z' ⁱⁿᵗ z'_ir)) (v':=VInt (z'0 ⁱⁿᵗ z'_ir0)) in H14; [|assumption]. now injection H14.
+Qed.
+
+
+Fact _determinist_c_exp_eval {T} : _determinist_exp_eval (@Empty_exp_sem T).
+Proof. easy. Qed.
+
+Definition determinist_c_exp_eval {T}:= determinist_exp_eval (@Empty_exp_sem T) _determinist_c_exp_eval.
+
+Fact Forall2_same_zargs { T : Set} : forall ev eargs zargs zargs0  exp_sem, 
+    _determinist_exp_eval exp_sem
+    -> List.Forall2 (@generic_exp_sem T exp_sem ev) eargs zargs 
+    -> List.Forall2 (@generic_exp_sem T exp_sem ev) eargs zargs0 -> zargs = zargs0.
+Proof.
+    intros ev eargs zargs zargs0 exp H  Hderiv. generalize dependent zargs0. induction Hderiv ; intros zargs0 H1.
+    - now inversion H1.
+    - destruct zargs0. inversion H1. apply List.Forall2_cons_iff in H1 as [H1 Hderiv2].
+        apply determinist_exp_eval in H0 ; [|assumption]. apply H0 in H1. subst. f_equal. clear H0.
+        now apply IHHderiv in Hderiv2.
+Qed.
+
+Fact determinist_stmt_eval {S T : Set}: 
+    forall ext_exp_sem ext_stmt_sem ext_stmt_vars, 
+    @_determinist_stmt_eval S T ext_exp_sem ext_stmt_sem -> 
+    _determinist_stmt_eval ext_exp_sem (@generic_stmt_sem S T ext_exp_sem ext_stmt_sem ext_stmt_vars).
+Proof with auto. 
+    intros ext_exp_sem ext_stmt_sem ext_stmt_vars Hds Hde f s ev ev' Hderiv. induction Hderiv ; intros.
+    - inversion H... 
+    - inversion H2 ; subst... repeat f_equal.  apply determinist_exp_eval in H8... specialize (H8 z). apply H8 in H1. now inversion H1.
+    - inversion H1 ; subst...  apply determinist_exp_eval in H6... destruct H as [H []]. apply H6 in H. now inversion H.
+    - inversion H1 ; subst... apply determinist_exp_eval in H... destruct H6 as [H2 []]. apply H in H2. now inversion H2.
+    - inversion H0... 
+    - inversion H1 ; subst... apply IHHderiv in H4. subst. apply IHHderiv0 in H6. now subst. 
+    - inversion H5 ; subst. 
+       (* same args, same body *) 
+            rewrite H10 in H0. injection H0 as H0. subst.
+            (* same args eval *) 
+            assert (zargs = zargs0). {
+                pose proof (@Forall2_same_zargs T ev eargs vargs vargs0 ext_exp_sem Hde H1 H11) as H0. unfold vargs,vargs0 in H0.
+                apply list_map_id_eq in H0. assumption. unfold Injective. intros x y H7. now inversion H7. 
+            }
+            subst. apply IHHderiv in H12. subst. rewrite H4 in H15. injection H15 as H15. now subst.
+    - inversion H3.  subst.  rewrite H7 in H0. injection H0 as Eq1. subst. 
+             assert (zargs = zargs0). {
+                pose proof (@Forall2_same_zargs T ev eargs vargs vargs0 ext_exp_sem Hde H1 H8) as H0. unfold vargs,vargs0 in H0.
+                apply list_map_id_eq in H0. assumption. unfold Injective. intros x y Heq. now inversion Heq. 
+             }
+             subst.
+            apply IHHderiv in H10. now subst.
+    - inversion H0 ; subst... apply determinist_exp_eval in H... apply H in H2. injection H2 as H2. now subst.
+    - inversion H1...
+    - inversion H0. subst. unfold _determinist_stmt_eval in Hds. eapply Hds... apply H. apply H2.
+Qed.
+
+Fact _determinist_c_stmt_eval {S T} : @_determinist_stmt_eval S T Empty_exp_sem Empty_stmt_sem. easy. Qed.
+Definition determinist_c_stmt_eval {S T} := determinist_stmt_eval Empty_exp_sem Empty_stmt_sem Empty_ext_stmt_vars (@_determinist_c_stmt_eval S T).
+
